# Khan/khan-exercises

Solved issue #32130.

1 parent a1978a3 commit d3ab2049396b8311c276a06a6208eb2367bf6c1c mirandaconrado committed Oct 20, 2012
Showing with 52 additions and 44 deletions.
1. +52 −44 exercises/pythagorean_identities.html
 @@ -182,12 +182,18 @@
Plugging into our expression, we get
-

+

\qquad + (IDENT)(FUNC) + = + (EQUIV)(FUNC) +

-

+

\qquad + \dfrac{IDENT}{FUNC} + = + \dfrac{EQUIV}{FUNC} +

@@ -197,13 +203,17 @@ , so we can plug that in to get

\qquad + (EQUIV)(FUNC) + = \left(EQUIV\right) \left(FUNC_SIMP\right)

-

\qquad + \dfrac{EQUIV}{FUNC} + = + \dfrac{EQUIV}{FUNC_SIMP}

@@ -217,7 +227,7 @@ random() < 0.5 random() < 0.5 - TAN ? ["1 + \\tan^2\\theta", "\\sec^2\\theta"] + TAN ? ["\\tan^2\\theta + 1", "\\sec^2\\theta"] : ["\\sec^2\\theta-1", "\\tan^2\\theta"] @@ -304,7 +314,7 @@ + \dfrac{\cos^2\theta}{\cos^2\theta} = \dfrac{1}{\cos^2\theta}

- \qquad 1 + \tan^2\theta = \sec^2\theta + \qquad \tan^2\theta + 1 = \sec^2\theta

@@ -313,14 +323,17 @@ Plugging into our expression, we get

\qquad + (IDENT)(FUNC) + = \left(EQUIV\right) \left(FUNC\right)

\qquad - \dfrac{EQUIV} - {FUNC} + \dfrac{IDENT}{FUNC} + = + \dfrac{EQUIV}{FUNC}

@@ -334,18 +347,18 @@

-

\qquad + \left(FUNC\right) + = \left(EQUIV_SIMP\right) \left(FUNC_SIMP\right)

-

-

+

\qquad + \dfrac{EQUIV}{FUNC} + = + \dfrac{EQUIV_SIMP}{FUNC_SIMP} +

@@ -357,21 +370,17 @@

-

\qquad + \left(FUNC\right) + = \left(EQUIV_SIMP\right) \left(FUNC_SIMP\right)

\qquad - \dfrac{EQUIV} - {FUNC_SIMP} -

-

\qquad - \dfrac{EQUIV_SIMP} - {FUNC_SIMP} + \dfrac{EQUIV}{FUNC} + = + \dfrac{EQUIV_SIMP}{FUNC_SIMP}

@@ -484,14 +493,17 @@ Plugging into our expression, we get

\qquad + (IDENT)(FUNC) + = \left(EQUIV\right) \left(FUNC\right)

\qquad - \dfrac{EQUIV} - {FUNC} + \dfrac{IDENT}{FUNC} + = + \dfrac{EQUIV}{FUNC}

@@ -505,18 +517,18 @@

-

\qquad + \left(FUNC\right) + = \left(EQUIV_SIMP\right) \left(FUNC_SIMP\right)

-

-

+

\qquad + \dfrac{EQUIV}{FUNC} + = + \dfrac{EQUIV_SIMP}{FUNC_SIMP} +

@@ -528,21 +540,17 @@

-

\qquad + \left(FUNC\right) + = \left(EQUIV_SIMP\right) \left(FUNC_SIMP\right)

\qquad - \dfrac{EQUIV} - {FUNC_SIMP} -

-

\qquad - \dfrac{EQUIV_SIMP} - {FUNC_SIMP} + \dfrac{EQUIV}{FUNC} + = + \dfrac{EQUIV_SIMP}{FUNC_SIMP}